Add decidable equality to Extset and Extmap, major refactor
Prove lemmas about canonicity and equality predicates
To do this, need to enforce key, value invariant
Change map to enforce invariant, prove for all functions
Push through to Set
TaggedType is now Countable

src/util/CoqUtil.v
@@ -159,3 +159,20 @@ Fixpoint list_eqb {A: Type} (eq: A -> A -> bool) (l1 l2: list A) : bool :=
   | nil, nil => true
   | _, _ => false
   end.
+
+Lemma list_eqb_eq {A: Type} {eq: A -> A -> bool} 
+  (Heq: forall x y, x = y <-> eq x y = true)
+  l1 l2:
+  l1 = l2 <-> list_eqb eq l1 l2 = true.
+Proof.
+  revert l2. induction l1 as [|h1 t1]; simpl;
+  intros [| h2 t2]; simpl; auto; try solve[split; auto; discriminate].
+  rewrite andb_true_iff, <- Heq, <- IHt1.
+  split; intros Hht; inversion Hht; subst; auto.
+Qed.
+
+Definition isSome {A: Type} (o: option A) : bool :=
+  match o with
+  | Some _ => true
+  | _ => false
+  end.
